concurrency/node-replication/FlatCombiner.i.dfy
@@ -1,0 +1,500 @@
+include "../framework/AsyncSSM.s.dfy"
+include "../../lib/Lang/NativeTypes.s.dfy"
+include "../../lib/Base/Option.s.dfy"
+include "Constants.i.dfy"
+include "../framework/Rw.i.dfy"
+include "../../lib/Base/Maps.i.dfy"
+
+module FlatCombiner refines Rw {
+  import opened RequestIds
+  import opened Constants
+  import Maps
+
+  type Key(!new) = nat
+  type StoredType(!new) = nat
+
+  datatype Elem = Elem(ghost rid: nat)
+
+  datatype FCClientState =
+    | FCClientIdle
+    | FCClientWaiting(ghost rid: RequestId)
+
+  datatype FCSlotState =
+    | FCEmpty
+    | FCRequest(ghost rid: RequestId)
+    | FCInProgress(ghost rid: RequestId)
+    | FCResponse(ghost rid: RequestId)
+
+  datatype FCCombinerState =
+    // no 'idle' state - just use Collecting([])
+    | FCCombinerCollecting(ghost elems: seq<Option<Elem>>)
+    | FCCombinerResponding(ghost elems: seq<Option<Elem>>, ghost idx: nat)
+
+  datatype M = M(
+    ghost clients: map<nat, FCClientState>,
+    ghost slots: map<nat, FCSlotState>,
+    ghost combiner: Option<FCCombinerState>
+  ) | Fail
+
+
+  /*
+   * ============================================================================================
+   * Invariant
+   * ============================================================================================
+   */
+
+  predicate ClientsComplete(c: map<nat, FCClientState>) {
+    && (forall i : nat | i in c :: 0 <= i < (MAX_THREADS_PER_REPLICA as nat))
+    && (forall i : nat | 0 <= i < (MAX_THREADS_PER_REPLICA as nat) :: i in c)
+  }
+
+  predicate SlotsComplete(s: map<nat, FCSlotState>) {
+    && (forall i : nat | i in s :: 0 <= i < (MAX_THREADS_PER_REPLICA as nat))
+    && (forall i : nat | 0 <= i < (MAX_THREADS_PER_REPLICA as nat) :: i in s)
+  }
+
+  predicate Complete(x: M) {
+    && x.M?
+    && x.combiner.Some?
+    && ClientsComplete(x.clients)
+    && SlotsComplete(x.slots)
+  }
+
+  predicate ClientIdle_SlotEmtpy(x: M)
+    requires Complete(x)
+  {
+    // the slot must be empty if the client is idling, and it's not empty if the client is waiting
+    && (forall i : nat | i in x.clients :: x.clients[i].FCClientIdle? <==> x.slots[i].FCEmpty?)
+  }
+
+  predicate ClientWaiting_RequestId(x: M)
+    requires Complete(x)
+    requires ClientIdle_SlotEmtpy(x)
+  {
+    // forall waiting clients, the request id in the slots must match
+    && (forall i : nat | i in x.clients && x.clients[i].FCClientWaiting? :: x.clients[i].rid == x.slots[i].rid)
+  }
+
+  predicate CombinerState_Elems(x: M)
+    requires Complete(x)
+  {
+    // the number of elements must not exceed the number of threads
+    && (|x.combiner.value.elems| <= MAX_THREADS_PER_REPLICA as nat)
+    && (x.combiner.value.FCCombinerResponding? ==>
+        (&& |x.combiner.value.elems| == MAX_THREADS_PER_REPLICA as nat
+        && x.combiner.value.idx <= |x.combiner.value.elems|
+        )
+      )
+  }
+
+  predicate CombinerState_RequestIds(x: M)
+    requires Complete(x)
+    requires CombinerState_Elems(x)
+  {
+    match x.combiner.value {
+      case FCCombinerCollecting(elems: seq<Option<Elem>>) => (
+        forall i : nat | 0 <= i < |x.combiner.value.elems| && x.combiner.value.elems[i].Some? :: (
+            x.slots[i].FCInProgress? || x.slots[i].FCResponse? ==> x.slots[i].rid == x.combiner.value.elems[i].value.rid
+        )
+      )
+      case FCCombinerResponding(elems: seq<Option<Elem>>, idx: nat) => (
+        forall i : nat | idx <= i < |x.combiner.value.elems| && x.combiner.value.elems[i].Some? :: (
+            x.slots[i].FCInProgress? || x.slots[i].FCResponse? ==> x.slots[i].rid == x.combiner.value.elems[i].value.rid
+        )
+      )
+    }
+  }
+
+  predicate Inv(x: M) {
+    && Complete(x)
+    && ClientIdle_SlotEmtpy(x)
+    && ClientWaiting_RequestId(x)
+    && CombinerState_Elems(x)
+    && CombinerState_RequestIds(x)
+  }
+
+
+  /*
+   * ============================================================================================
+   * Initialization
+   * ============================================================================================
+   */
+
+  predicate Init(s: M) {
+    s == M(
+      map x : nat | 0 <= x < (MAX_THREADS_PER_REPLICA as nat) :: x := FCClientIdle,
+      map x : nat | 0 <= x < (MAX_THREADS_PER_REPLICA as nat) :: x := FCEmpty,
+      Some(FCCombinerCollecting([]))
+    )
+  }
+
+  lemma InitImpliesInv(x: M)
+    requires Init(x)
+    ensures Inv(x)
+  {
+  }
+
+   /*
+   * ============================================================================================
+   * Dot
+   * ============================================================================================
+   */
+
+  function dot(x: M, y: M) : M {
+    if (
+      && x.M?                &&  y.M?
+      && !(x.combiner.Some?  &&  y.combiner.Some?)
+      && (x.slots.Keys       !!  y.slots.Keys)
+      && (x.clients.Keys     !!  y.clients.Keys)
+    )
+    then
+      M(
+        Maps.MapUnionPreferB(x.clients, y.clients),
+        Maps.MapUnionPreferB(x.slots, y.slots),
+        if x.combiner.Some? then x.combiner else y.combiner
+      )
+    else
+      Fail
+  }
+
+  function unit() : M {
+    M(map[], map[], None)
+  }
+
+  lemma dot_unit(x: M)
+  ensures dot(x, unit()) == x
+  {
+    assert unit().M?;
+    assert dot(unit(), unit()).M?;
+    assert dot(unit(), unit()) == unit();
+    assert dot(x, unit()) == x;
+  }
+
+  lemma commutative(x: M, y: M)
+  ensures dot(x, y) == dot(y, x)
+  {
+    if dot(x, y) == Fail {
+      assert dot(x, y) == dot(y, x);
+    } else {
+      assert dot(x, y) == dot(y, x);
+    }
+  }
+
+  lemma associative(x: M, y: M, z: M)
+  ensures dot(x, dot(y, z)) == dot(dot(x, y), z)
+  {
+    if dot(x, dot(y, z)) == Fail {
+      assert dot(x, dot(y, z)) == dot(dot(x, y), z);
+    } else {
+      assert dot(x, dot(y, z)) == dot(dot(x, y), z);
+    }
+  }
+
+
+  /*
+   * ============================================================================================
+   * Interpretation Function
+   * ============================================================================================
+   */
+  // probably don't need?
+  function I(x: M) : Option<StoredType> {
+    None
+  }
+
+
+  /*
+   * ============================================================================================
+   * Guards
+   * ============================================================================================
+   */
+
+  predicate CombinerValid(m: M) {
+    && m.M?
+    && m.combiner.Some?
+  }
+
+  predicate CombinerIsCollecting(m: M)
+    requires CombinerValid(m)
+  {
+    && m.combiner.value.FCCombinerCollecting?
+    && |m.combiner.value.elems| < MAX_THREADS_PER_REPLICA as nat
+  }
+
+  predicate CombinerIsCollectingDone(m: M)
+    requires CombinerValid(m)
+  {
+    && m.combiner.value.FCCombinerCollecting?
+    && |m.combiner.value.elems| == MAX_THREADS_PER_REPLICA as nat
+  }
+
+  predicate CombinerIsResponding(m: M)
+    requires CombinerValid(m)
+  {
+     && m.combiner.value.FCCombinerResponding?
+     && m.combiner.value.idx < |m.combiner.value.elems|
+  }
+
+  predicate CombinerIsRespondingDone(m: M)
+    requires CombinerValid(m)
+  {
+     && m.combiner.value.FCCombinerResponding?
+     && m.combiner.value.idx == |m.combiner.value.elems|
+  }
+
+  predicate ClientIdle(m: M, tid: nat)
+    requires m.M?
+  {
+    && tid in m.clients
+    && m.clients[tid].FCClientIdle?
+  }
+
+  predicate ClientWaiting(m: M, tid:nat)
+    requires m.M?
+  {
+    && tid in m.clients
+    && m.clients[tid].FCClientWaiting?
+  }
+
+  predicate SlotIsEmpty(m: M, tid: nat)
+    requires m.M?
+  {
+    && tid in m.slots
+    && m.slots[tid].FCEmpty?
+  }
+
+  predicate SlotHasRequest(m: M, tid: nat)
+    requires m.M?
+  {
+    && tid in m.slots
+    && m.slots[tid].FCRequest?
+  }
+
+  predicate SlotInProgress(m: M, tid: nat)
+    requires m.M?
+  {
+    && tid in m.slots
+    && m.slots[tid].FCRequest?
+  }
+
+  predicate SlotHasResponse(m: M, tid: nat)
+    requires m.M?
+  {
+    && tid in m.slots
+    && m.slots[tid].FCRequest?
+  }
+
+  /*
+   * ============================================================================================
+   * State Transitions
+   * ============================================================================================
+   */
+
+  // -------------------------------- fc_initialize ---------------------------------------------
+
+  // TODO?
+
+  // -------------------------------- combiner_collect ------------------------------------------
+
+  // TODO: break the up into two transitions?
+  predicate CombinerDoCollectEmpty(m: M, m': M) {
+    && m.M?
+    && CombinerValid(m)
+    && CombinerIsCollecting(m)
+
+    // get the thread id as the current number of elements in the combiner elements
+    && var tid := |m.combiner.value.elems|;
+
+    // the slot was empty
+    && SlotIsEmpty(m, tid)
+
+    // add a None to the collected elements
+    && m' == m.(combiner := Some(FCCombinerCollecting(m.combiner.value.elems + [None])))
+  }
+
+  lemma CombinerDoCollectEmpty_is_transition(m: M, m': M)
+  requires CombinerDoCollectEmpty(m, m')
+  ensures transition(m, m')
+  {
+
+  }
+
+  // -------------------------------- combiner_collect ------------------------------------------
+
+  predicate CombinerDoCollectRequest(m: M, m': M) {
+    && m.M?
+    && CombinerValid(m)
+    && CombinerIsCollecting(m)
+
+    // get the thread id as the current number of elements in the combiner elements
+    && var tid := |m.combiner.value.elems|;
+
+    // the slot had a request
+    && SlotHasRequest(m, tid)
+
+    // mark the slot as in progress, and add the request Id to the elements
+    && m' == m.(
+      combiner := Some(FCCombinerCollecting(m.combiner.value.elems + [Some(Elem(m.slots[tid].rid))])),
+      slots := m.slots[tid := FCInProgress(m.slots[tid].rid)]
+    )
+  }
+
+  lemma CombinerDoCollectRequest_is_transition(m: M, m': M)
+  requires CombinerDoCollectRequest(m, m')
+  ensures transition(m, m')
+  {
+    forall p: M | Inv(dot(m, p))
+      ensures Inv(dot(m', p))
+      && I(dot(m, p)) == I(dot(m', p))
+    {
+
+    }
+  }
+
+
+  // -------------------------------- combiner_goto_responding ----------------------------------
+
+  predicate CombinerGoToResponding(m: M, m': M) {
+    && m.M?
+    && CombinerValid(m)
+    && CombinerIsCollectingDone(m)
+
+    // keep the elements, set the index to 0
+    && m' == m.(combiner := Some(FCCombinerResponding(m.combiner.value.elems, 0)))
+  }
+
+  lemma CombinerGoToResponding_is_transition(m: M, m': M)
+    requires CombinerGoToResponding(m, m')
+    ensures transition(m, m')
+  {
+
+  }
+
+
+  // -------------------------------- combiner_response_skip ------------------------------------
+
+  predicate CombinerDoResponseSkip(m: M, m': M)
+  {
+    && m.M?
+    && CombinerValid(m)
+    && CombinerIsResponding(m)
+
+    // the current thread we're responding to
+    && var tid := m.combiner.value.idx;
+
+    // the element was none, so nothing to be done
+    && m.combiner.value.elems[tid].None?
+
+    && m' == m.(combiner := Some(FCCombinerResponding(m.combiner.value.elems, tid + 1)))
+  }
+
+  lemma CombinerDoResponseSkip_is_transition(m: M, m': M)
+    requires CombinerDoResponseSkip(m, m')
+    ensures transition(m, m')
+  {
+
+  }
+
+  // -------------------------------- combiner_response -----------------------------------------
+
+  predicate CombinerDoResponse(m: M, m': M)
+  {
+    && m.M?
+    && CombinerValid(m)
+    && CombinerIsResponding(m)
+    // the current thread we're responding to
+    && var tid := m.combiner.value.idx;
+
+    // the element was none, so nothing to be done
+    && m.combiner.value.elems[tid].Some?
+
+    // the slot state must be in progress
+    && tid in m.slots && m.slots[tid].FCInProgress?
+
+    && m' == m.(
+      combiner := Some(FCCombinerResponding(m.combiner.value.elems, tid + 1)),
+      slots := m.slots[tid := FCResponse(m.slots[tid].rid)]
+    )
+  }
+
+  lemma CombinerDoResponse_is_transition(m: M, m': M)
+    requires CombinerDoResponse(m, m')
+    ensures transition(m, m')
+  {
+
+  }
+
+  // -------------------------------- combiner_goto_collecting ----------------------------------
+
+  predicate CombinerGoToCollecting(m: M, m': M)
+  {
+    && m.M?
+    && CombinerValid(m)
+    && CombinerIsRespondingDone(m)
+
+    && m' == m.(combiner := Some(FCCombinerCollecting([])))
+  }
+
+  lemma CombinerGoToCollecting_is_transition(m: M, m': M)
+    requires CombinerGoToCollecting(m, m')
+    ensures transition(m, m')
+  {
+
+  }
+
+
+  // -------------------------------- fc_send ---------------------------------------------------
+
+  predicate FCSend(m: M, m': M, tid: nat, rid: RequestId) {
+    && m.M?
+    && ClientIdle(m, tid)
+
+    // we're modifying this
+    && tid in m.slots
+
+    && m' == m.(
+      clients := m.clients[tid := FCClientWaiting(rid)],
+      slots  := m.slots[tid := FCRequest(rid)])
+  }
+
+  lemma FCSend_is_transition(m: M, m': M, tid: nat, rid: RequestId)
+    requires FCSend(m, m', tid, rid)
+    ensures transition(m, m')
+  {
+    forall p: M | Inv(dot(m, p))
+      ensures Inv(dot(m', p))
+      && I(dot(m, p)) == I(dot(m', p))
+    {
+     assume false;
+    }
+  }
+
+  // -------------------------------- fc_recv ---------------------------------------------------
+
+
+  predicate FCRecv(m: M, m': M, tid: nat, rid: RequestId) {
+    && m.M?
+    && ClientWaiting(m, tid)
+
+    && SlotHasResponse(m, tid)
+
+    // && rid == m.clients[tid].rid
+
+    && m' == m.(
+      clients := m.clients[tid := FCClientIdle],
+      slots  := m.slots[tid := FCEmpty])
+  }
+
+  lemma FCRecv_is_transition(m: M, m': M, tid: nat, rid: RequestId)
+    requires FCRecv(m, m', tid, rid)
+    ensures transition(m, m')
+  {
+    forall p: M | Inv(dot(m, p))
+      ensures Inv(dot(m', p))
+      && I(dot(m, p)) == I(dot(m', p))
+    {
+      assert (CombinerState_RequestIds(dot(m', p)));
+    }
+  }
+
+}
+
